state/Witnessable.fst
@@ -8,21 +8,15 @@ open FStar.Monotonic.Heap
 open MST.Repr
 open MST.Tot
 
-type ref_heap_pred =
-  #a:Type -> #rel:FStar.Preorder.preorder a -> mref a rel -> heap -> Type0
-
-type ref_heap_pred_stable =
-  pred:ref_heap_pred{forall (a:Type) rel (x:mref a rel) h0 h1. pred x h0 /\ h0 `heap_rel` h1 ==> pred x h1}
-
 class witnessable (t:Type) = {
   satisfy : t -> (#a:_ -> #rel:_ -> mref a rel -> Type0) -> Type0;
-  satisfy_on_heap : t -> heap -> ref_heap_pred -> Type0;
+  satisfy_on_heap : t -> heap -> mref_heap_pred -> Type0;
 
-  satisfy_on_heap_monotonic : x:t -> pred:ref_heap_pred_stable -> h0:heap -> h1:heap ->
+  satisfy_on_heap_monotonic : x:t -> pred:mref_heap_stable_pred -> h0:heap -> h1:heap ->
     Lemma (requires (h0 `heap_rel` h1 /\ satisfy_on_heap x h0 pred))
           (ensures (satisfy_on_heap x h1 pred));
 
-  pwitness : x:t -> pred:ref_heap_pred_stable -> ST (precall:(unit -> ST unit (fun _ -> True) (fun h0 _ h1 -> h0 == h1 /\ satisfy_on_heap x h1 pred)))
+  pwitness : x:t -> pred:mref_heap_stable_pred -> ST (precall:(unit -> ST unit (fun _ -> True) (fun h0 _ h1 -> h0 == h1 /\ satisfy_on_heap x h1 pred)))
     (requires (fun h0 -> satisfy_on_heap x h0 pred))
     (ensures (fun h0 _ h1 -> h0 == h1));
 }
@@ -97,7 +91,7 @@ let rec forall_in_list (l:list 'a) (pred:'a -> Type0) : Type0 =
   | [] -> True
   | hd::tl -> pred hd /\ forall_in_list tl pred
 
-val list_satisfy_on_heap_monotonic : #t:_ -> {| c:witnessable t |} -> l:list t -> pred:ref_heap_pred_stable -> h0:heap -> h1:heap ->
+val list_satisfy_on_heap_monotonic : #t:_ -> {| c:witnessable t |} -> l:list t -> pred:mref_heap_stable_pred -> h0:heap -> h1:heap ->
   Lemma (requires (h0 `heap_rel` h1 /\ forall_in_list l (fun x -> c.satisfy_on_heap x h0 pred)))
         (ensures (forall_in_list l (fun x -> c.satisfy_on_heap x h1 pred)))
 let rec list_satisfy_on_heap_monotonic #_ #c l pred h0 h1 =
